WIP verilog semantics sort

vera/Common.v
@@ -493,11 +493,83 @@ Lemma disjoint_r_intro A (l r : list A) : forall x,
   ~ In x l.
 Proof. unfold disjoint. setoid_rewrite Forall_forall. firstorder. Qed.
 
-(* Just checking that typeclasses eauto can indeed figure out DecProp (disjoint l r) *)
+(* TODO: Move me to common *)
+Lemma disjoint_app_l {A} (l1 l2 l3 : list A):
+  disjoint (l1 ++ l2) l3 ->
+  disjoint l1 l3.
+Proof.
+  unfold disjoint.
+  rewrite ! List.Forall_app.
+  crush.
+Qed.
+
+(* TODO: Move me to common *)
+Lemma disjoint_app_r {A} (l1 l2 l3 : list A):
+  disjoint (l1 ++ l2) l3 ->
+  disjoint l2 l3.
+Proof.
+  unfold disjoint.
+  rewrite ! List.Forall_app.
+  crush.
+Qed.
+
+(* TODO: Move me to common *)
+Lemma disjoint_app {A} (l1 l2 l3 : list A):
+  disjoint (l1 ++ l2) l3 ->
+  disjoint l1 l3 /\ disjoint l2 l3.
+Proof.
+  unfold disjoint.
+  rewrite ! List.Forall_app.
+  crush.
+Qed.
+
+(* TODO: Move me to common *)
+Lemma disjoint_sym {A} (l1 l2 : list A):
+  disjoint l1 l2 <->
+  disjoint l2 l1.
+Proof.
+  unfold disjoint.
+  rewrite ! List.Forall_forall.
+  crush.
+Qed.
+
+(* Checking that typeclasses eauto can indeed figure out DecProp (disjoint l r) *)
 Goal (forall (l r : list nat), DecProp (disjoint l r)). typeclasses eauto. Qed.
 
 Definition list_subset {A} (sub sup : list A) : Prop :=
   Forall (fun x => In x sup) sub.
 
-(* Same for subset *)
+Definition permutation {A} (l1 l2 : list A) : Prop :=
+  forall x, List.In x l1 <-> List.In x l2.
+
+Lemma permutation_nil {A} (l : list A) : permutation [] l -> l = [].
+Proof.
+  unfold permutation. intros H.
+  destruct l; [reflexivity|].
+  exfalso. eapply List.in_nil.
+  eapply H. constructor. reflexivity.
+Qed.
+
+Lemma permutation_cons {A} a (l1 l2 : list A) :
+  permutation (a :: l1) l2 ->
+  (List.In a l2 /\ List.Forall (fun x => List.In x l2) l1).
+Proof.
+  unfold permutation. intros H.
+  rewrite List.Forall_forall.
+  destruct l1; crush.
+Qed.
+
+Lemma permutation_refl {A} (l : list A) : permutation l l.
+Proof. crush. Qed.
+
+Lemma permutation_sym {A} (l1 l2 : list A) : permutation l1 l2 <-> permutation l2 l1.
+Proof. crush. Qed.
+
+Lemma permutation_trans {A} (l1 l2 l3 : list A) :
+  permutation l1 l2 ->
+  permutation l2 l3 ->
+  permutation l1 l3.
+Proof. crush. Qed.
+
+(* Checking that typeclasses eauto can indeed figure out DecProp (list_subset l r) *)
 Goal (forall (sub sup : list nat), DecProp (list_subset sub sup)). typeclasses eauto. Qed.
